linked lists - some methods and examples

state/LinkedListIFC.fst
@@ -8,16 +8,67 @@ open IFC.Heap.ST
 open STLC
 open TargetLangIFC
 
-// noeq type linkedList (a: Type0) : Type0 =
-//    | Nil
-//    | Cons of a * ref (linkedList a)
+noeq type linkedList (a: Type0) : Type0 =
+    | Nil
+    | Cons of a * ref (linkedList a)
 
-type node (#t:Type) {| c:target_lang t |} (v:t) (r: ref t) = (v, r)
+// TODO: separate the current invariant into two invariants (and shallowly_witnessed into two parts accordingly)
 
-// val empty_ll: IST (ref int) (requires _ -> True) (ensures _ _ _ -> True)
-// let empty = 
-//     let head: option (ref int) = alloc 0 in
-//     head := None;
-//     head
+instance target_lang_linkedList (t1:Type) {| c1:target_lang t1 |} : target_lang (linkedList t1) = {
+  shallowly_witnessed = (fun x ->
+    match x with
+    | Nil -> True
+    // is witnessed (is_low_pred tl) needed?
+    | Cons (h, tl) -> c1.shallowly_witnessed h /\ is_mm tl = false /\ witnessed (contains_pred tl) /\ witnessed (is_low_pred tl)); 
+}
 
-// val insert
+let tail (a: Type0) (l: linkedList a) {| c1:target_lang a |} : IST (linkedList a)
+    (requires (fun h -> shallowly_witnessed l))
+    (ensures fun _ _ _ -> True) = 
+      match l with
+      | Nil -> Nil
+      | Cons (h, tl) -> !tl
+
+let append (a: Type0) (l: linkedList a) (v: a) {| c:target_lang a |}: ST (linkedList a)
+    (requires (fun _ -> True))
+    (ensures fun _ _ _ -> True) = 
+    let r: ref (linkedList a) = alloc l in 
+    Cons (v, r)
+
+let rec length (a: Type0) (l: linkedList a) {| c:target_lang a |} : IST nat 
+       (requires (fun h -> shallowly_witnessed l))
+       (ensures fun _ _ _ -> True) =
+       let h0 = get() in
+        match l with 
+         | Nil -> 0
+         | Cons (h, tlref) -> 
+           let tl = !tlref in
+             eliminate forall (a:Type) (c:target_lang a) (r:ref a). witnessed (is_low_pred r) ==>
+            c.shallowly_witnessed (sel h0 r) with (linkedList a) (solve) tlref;
+           1 + length a tl #c
+
+
+// val insert (a: Type0) {| c:target_lang a |} : linkedList a -> ref (linkedList a) -> v: a -> St (linkedList a)
+// let insert a l r v = 
+
+// examples
+
+let empty_ll: linkedList nat = Nil
+
+let ll1 () : ST (linkedList nat) (requires fun _ -> True) (ensures fun _ _ _ -> True) =
+     let r: ref(linkedList nat) = alloc Nil in 
+     Cons (13, r)
+
+let ll2 () : ST (linkedList nat) (requires fun _ -> True) (ensures fun _ _ _ -> True) =
+     let x = alloc Nil in 
+     let y = alloc (Cons (31, x)) in
+     let z = alloc (Cons (23, y)) in
+     Cons(23, z)
+
+let cycle_length3 () : ST (linkedList nat) (requires fun _ -> True) (ensures fun _ _ _ -> True) =
+    let x = alloc Nil in 
+    let y = alloc (Cons (7, x)) in
+    let z = alloc (Cons (5, y)) in 
+    gst_witness (contains_pred x);
+    write x (Cons(2, z));
+    Cons (2, z)
